cfrontend/Ctyping.v
@@ -426,10 +426,12 @@ Inductive wt_rvalue : expr -> Prop :=
     wt_rvalue (Efailstop ty)
 
 with wt_lvalue : expr -> Prop :=
-| wt_Eloc: forall ofs pt bf ty,
-    wt_lvalue (Eloc ofs pt bf ty)
-| wt_Efloc: forall b pt ty,
-    wt_lvalue (Efloc b pt ty)
+| wt_Eloc_mem: forall ofs pt bf ty,
+    wt_lvalue (Eloc (Lmem ofs pt bf) ty)
+| wt_Eloc_tmp: forall b ty,
+    wt_lvalue (Eloc (Ltmp b) ty)
+| wt_Eloc_fun: forall b pt tyargs tyres cconv,
+    wt_lvalue (Eloc (Lfun b pt) (Tfunction tyargs tyres cconv))
 | wt_Evar: forall x ty,
     e!x = Some ty ->
     wt_lvalue (Evar x ty)
@@ -458,8 +460,7 @@ Definition wt_expr_kind (k: kind) (a: expr) :=
 
 Definition expr_kind (a: expr) : kind :=
   match a with
-  | Eloc _ _ _ _ => LV
-  | Efloc _ _ _ => LV
+  | Eloc _ _ => LV
   | Evar _ _ => LV
   | Ederef _ _ => LV
   | Efield _ _ _ => LV
@@ -615,7 +616,7 @@ Fixpoint check_arguments (el: exprlist) (tyl: typelist) : res unit :=
 
 Definition check_rval (e: expr) : res unit :=
   match e with
-  | Eloc _ _ _ _ | Efloc _ _ _ | Evar _ _ | Ederef _ _ | Efield _ _ _ =>
+  | Eloc _ _ | Evar _ _ | Ederef _ _ | Efield _ _ _ =>
       Error (msg "not a r-value")
   | _ =>
       OK tt
@@ -623,7 +624,7 @@ Definition check_rval (e: expr) : res unit :=
 
 Definition check_lval (e: expr) : res unit :=
   match e with
-  | Eloc _ _ _ _ | Evar _ _ | Ederef _ _ | Efield _ _ _ =>
+  | Eloc _ _ | Evar _ _ | Ederef _ _ | Efield _ _ _ =>
       OK tt
   | _ =>
       Error (msg "not a l-value")
@@ -871,10 +872,8 @@ Fixpoint retype_expr (ce: composite_env) (e: typenv) (a: expr) : res expr :=
       do r1' <- retype_expr ce e r1; do rl' <- retype_exprlist ce e rl; ecall r1' rl'
   | Ebuiltin ef tyargs rl tyres =>
       do rl' <- retype_exprlist ce e rl; ebuiltin ef tyargs rl' tyres
-  | Eloc _ _ _ _ =>
+  | Eloc _ _ =>
       Error (msg "Eloc in source")
-  | Efloc _ _ _ =>
-      Error (msg "Efloc in source")
   | Eparen _ _ _ =>
       Error (msg "Eparen in source")
   | Efailstop ty =>
@@ -1843,85 +1842,88 @@ Proof.
 Qed.
 
 Lemma wt_rred:
-  forall ge tenv PCT a m t PCT' a' m',
-  rred ge PCT a m t PCT' a' m' -> wt_rvalue (snd ge) tenv a -> wt_rvalue (snd ge) tenv a'.
+  forall ge tyenv PCT a te m t PCT' a' te' m',
+    rred ge PCT a te m t PCT' a' te' m' -> wt_rvalue (snd ge) tyenv a -> wt_rvalue (snd ge) tyenv a'.
 Proof.
   induction 1; intros WT; inversion WT.
-- (* valof *) simpl in *. constructor. eapply wt_deref_loc in H; eauto.
-- (* addrof *) unfold Vofptrsize; destruct Archi.ptr64; constructor; auto with ty. 
-- (* unop *) simpl in H5. inv H2. constructor. eapply pres_sem_unop; inv H3; eauto.
-- (* binop *)
-  simpl in H7. inv H4. inv H6. constructor. eapply pres_sem_binop; eauto.
-- (* cast *) inv H2. constructor. eapply pres_sem_cast; eauto.
-- (* sequand true *) subst. constructor. auto. apply wt_bool_cast; auto.
-  red; intros. inv H0; auto with ty.
-- (* sequand false *) constructor. auto with ty.
-- (* seqor true *) constructor. auto with ty.
-- (* seqor false *) subst. constructor. auto. apply wt_bool_cast; auto.
-  red; intros. inv H0; auto with ty.
-- (* condition *) constructor. destruct b; auto. destruct b; auto. red; auto.
-- (* sizeof *)  unfold size_t, Vofptrsize; destruct Archi.ptr64; constructor; auto with ty.
-- (* alignof *)  unfold size_t, Vofptrsize; destruct Archi.ptr64; constructor; auto with ty.
-- (* assign *) inversion H6. constructor. eapply wt_assign_loc in H3; eauto. eapply pres_sem_cast; eauto. inv H8. auto.
-- (* assignop *) subst tyres l r. constructor. auto.
-  constructor. constructor. eapply wt_deref_loc in H; eauto.
-  auto. auto. auto.
-- (* postincr *) simpl in *. subst id0 l.
-  exploit wt_deref_loc; eauto. intros WTV1.
-  constructor.
-  constructor. auto. rewrite <- H1 in H6. constructor.
-  constructor; auto. constructor. constructor. auto with ty.
-  subst op. destruct id.
-  erewrite <- type_add_int32s by eauto. auto.
-  erewrite <- type_sub_int32s by eauto. auto.
-  simpl; auto.
-  constructor; auto.
-- (* comma *) auto.
-- (* paren *) inv H3. constructor. apply H5. eapply pres_sem_cast; inv H; eauto.
-- (* builtin *) subst. destruct H7 as [(A & B) | (A & B)].
-+ subst ty. destruct vres; simpl. auto with ty. 
-+ simpl in B. set (T := typ_of_type ty) in *. 
-  set (sg := mksignature (AST.Tint :: T :: T :: nil) T cc_default) in *.
-  assert (LK: lookup_builtin_function "__builtin_sel"%string sg = Some (BI_standard (BI_select T))).
-  { unfold sg, T; destruct ty as   [ | ? ? ? | ? | [] ? | ? ? | ? ? ? | ? ? ? | ? ? | ? ? ];
-    simpl; unfold Tptr; destruct Archi.ptr64; reflexivity. }
-  subst ef. red in H0. red in H0. rewrite LK in H0. inv H0. 
-  inv H. inv H8. inv H10. inv H11. simpl in H1.
-  assert (A: val_casted v1 type_bool) by (eapply cast_val_is_casted; eauto).
-  inv A. 
-  set (v' := if Int.eq n Int.zero then v4 else v2) in *.
-  constructor.
-  destruct (type_eq ty Tvoid).
-  subst. constructor.
-  destruct vargs0; try discriminate. simpl in H5. inv H5.
-  destruct vargs0; try discriminate. simpl in H10. inv H10.
-  destruct vargs0; try discriminate. simpl in H9. inv H9.
-  destruct vargs0; try discriminate.
-  inv H1.
-  assert (C: val_casted v' ty).
-  { unfold v'; destruct (Int.eq n Int.zero); eapply cast_val_is_casted; eauto. }
-  assert (EQ: Val.normalize v' T = v').
-  { apply Val.normalize_idem. apply val_casted_has_type; auto. }
-  unfold v' in EQ. rewrite EQ. apply wt_val_casted; auto.
+  - (* const *) constructor. auto.
+  - (* valof_mem *) simpl in *. constructor. eapply wt_deref_loc in H; eauto.
+  - (* valof_fun *) simpl in *. constructor. inv H0. constructor.
+  - (* valof_tmp *) simpl in *. constructor.
+  - (* addrof *) unfold Vofptrsize; destruct Archi.ptr64; constructor; auto with ty.
+  - (* unop *) simpl in H5. inv H2. constructor. eapply pres_sem_unop; inv H3; eauto.
+  - (* binop *)
+    simpl in H7. inv H4. inv H6. constructor. eapply pres_sem_binop; eauto.
+  - (* cast *) inv H2. constructor. eapply pres_sem_cast; eauto.
+  - (* sequand true *) subst. constructor. auto. apply wt_bool_cast; auto.
+    red; intros. inv H0; auto with ty.
+  - (* sequand false *) constructor. auto with ty.
+  - (* seqor true *) constructor. auto with ty.
+  - (* seqor false *) subst. constructor. auto. apply wt_bool_cast; auto.
+    red; intros. inv H0; auto with ty.
+  - (* condition *) constructor. destruct b; auto. destruct b; auto. red; auto.
+  - (* sizeof *)  unfold size_t, Vofptrsize; destruct Archi.ptr64; constructor; auto with ty.
+  - (* alignof *)  unfold size_t, Vofptrsize; destruct Archi.ptr64; constructor; auto with ty.
+  - (* assign *) inversion H6. constructor. eapply wt_assign_loc in H3; eauto. eapply pres_sem_cast; eauto. inv H8. auto.
+  - (* assignop *) subst tyres l r. constructor. auto.
+    constructor. constructor. eapply wt_deref_loc in H; eauto.
+    auto. auto. auto.
+  - (* postincr *) simpl in *. subst id0 l.
+    exploit wt_deref_loc; eauto. intros WTV1.
+    constructor.
+    constructor. auto. rewrite <- H2 in H7. constructor.
+    constructor; auto. constructor. constructor. auto with ty.
+    subst op. destruct id.
+    erewrite <- type_add_int32s by eauto. auto.
+    erewrite <- type_sub_int32s by eauto. auto.
+    simpl; auto.
+    constructor; auto.
+  - (* comma *) auto.
+  - (* paren *) inv H4. constructor. apply H6. eapply pres_sem_cast; inv H; eauto.
+  - (* builtin *) subst. destruct H7 as [(A & B) | (A & B)].
+    + subst ty. destruct vres; simpl. auto with ty. 
+    + simpl in B. set (T := typ_of_type ty) in *. 
+      set (sg := mksignature (AST.Tint :: T :: T :: nil) T cc_default) in *.
+      assert (LK: lookup_builtin_function "__builtin_sel"%string sg = Some (BI_standard (BI_select T))).
+      { unfold sg, T; destruct ty as   [ | ? ? ? | ? | [] ? | ? ? | ? ? ? | ? ? ? | ? ? | ? ? ];
+          simpl; unfold Tptr; destruct Archi.ptr64; reflexivity. }
+      subst ef. red in H0. red in H0. rewrite LK in H0. inv H0. 
+      inv H. inv H8. inv H10. inv H11. simpl in H1.
+      assert (A: val_casted v1 type_bool) by (eapply cast_val_is_casted; eauto).
+      inv A. 
+      set (v' := if Int.eq n Int.zero then v4 else v2) in *.
+      constructor.
+      destruct (type_eq ty Tvoid).
+      subst. constructor.
+      destruct vargs0; try discriminate. simpl in H5. inv H5.
+      destruct vargs0; try discriminate. simpl in H10. inv H10.
+      destruct vargs0; try discriminate. simpl in H9. inv H9.
+      destruct vargs0; try discriminate.
+      inv H1.
+      assert (C: val_casted v' ty).
+      { unfold v'; destruct (Int.eq n Int.zero); eapply cast_val_is_casted; eauto. }
+      assert (EQ: Val.normalize v' T = v').
+      { apply Val.normalize_idem. apply val_casted_has_type; auto. }
+      unfold v' in EQ. rewrite EQ. apply wt_val_casted; auto.
 Qed.
 
 Lemma wt_lred:
-  forall tenv ge e a m a' m',
-  lred ge e a m a' m' -> wt_lvalue (snd ge) tenv a -> wt_lvalue (snd ge) tenv a'.
+  forall tenv ge e a pct m a' m',
+    lred ge e a pct m a' m' -> wt_lvalue (snd ge) tenv a -> wt_lvalue (snd ge) tenv a'.
 Proof.
-  induction 1; intros WT; constructor.
+  induction 1; intros WT; try constructor.
 Qed.
 
 Lemma rred_same_type:
-  forall ge PCT a m t PCT' a' m',
-  rred ge PCT a m t PCT' a' m' -> typeof a' = typeof a.
+  forall ge e PCT a m t PCT' a' m',
+  rred ge e PCT a m t PCT' a' m' -> typeof a' = typeof a.
 Proof.
   induction 1; auto.
 Qed.
 
 Lemma lred_same_type:
-  forall ge e a m a' m',
-  lred ge e a m a' m' -> typeof a' = typeof a.
+  forall ge e a pct m a' m',
+  lred ge e a pct m a' m' -> typeof a' = typeof a.
 Proof.
   induction 1; auto.
 Qed.
